James C - abstracted out vars

isabelle/Chapter04.thy
@@ -5,7 +5,7 @@ begin
 datatype type = NumType | StrType
 
 datatype expr = 
-  Var nat
+  Var var
 | Num int
 | Str string
 | Plus expr expr
@@ -37,27 +37,27 @@ inductive_cases [elim!]: "typecheck gam (Cat e1 e2) t"
 inductive_cases [elim!]: "typecheck gam (Len e) t"
 inductive_cases [elim!]: "typecheck gam (Let e1 e2) t"
 
-primrec incr_from :: "nat => expr => expr"
-where "incr_from n (Var v) = Var (if v < n then v else Suc v)"
-    | "incr_from n (Num x) = Num x"
-    | "incr_from n (Str s) = Str s"
-    | "incr_from n (Plus e1 e2) = Plus (incr_from n e1) (incr_from n e2)"
-    | "incr_from n (Times e1 e2) = Times (incr_from n e1) (incr_from n e2)"
-    | "incr_from n (Cat e1 e2) = Cat (incr_from n e1) (incr_from n e2)"
-    | "incr_from n (Len e) = Len (incr_from n e)"
-    | "incr_from n (Let e1 e2) = Let (incr_from n e1) (incr_from (Suc n) e2)"
+primrec insert :: "var => expr => expr"
+where "insert n (Var v) = Var (incr n v)"
+    | "insert n (Num x) = Num x"
+    | "insert n (Str s) = Str s"
+    | "insert n (Plus e1 e2) = Plus (insert n e1) (insert n e2)"
+    | "insert n (Times e1 e2) = Times (insert n e1) (insert n e2)"
+    | "insert n (Cat e1 e2) = Cat (insert n e1) (insert n e2)"
+    | "insert n (Len e) = Len (insert n e)"
+    | "insert n (Let e1 e2) = Let (insert n e1) (insert (next n) e2)"
 
-primrec sub_from :: "nat => expr => expr"
-where "sub_from n (Var v) = Var (if v < n then v else v - 1)"
-    | "sub_from n (Num x) = Num x"
-    | "sub_from n (Str s) = Str s"
-    | "sub_from n (Plus e1 e2) = Plus (sub_from n e1) (sub_from n e2)"
-    | "sub_from n (Times e1 e2) = Times (sub_from n e1) (sub_from n e2)"
-    | "sub_from n (Cat e1 e2) = Cat (sub_from n e1) (sub_from n e2)"
-    | "sub_from n (Len e) = Len (sub_from n e)"
-    | "sub_from n (Let e1 e2) = Let (sub_from n e1) (sub_from (Suc n) e2)"
+primrec remove :: "var => expr => expr"
+where "remove n (Var v) = Var (subr n v)"
+    | "remove n (Num x) = Num x"
+    | "remove n (Str s) = Str s"
+    | "remove n (Plus e1 e2) = Plus (remove n e1) (remove n e2)"
+    | "remove n (Times e1 e2) = Times (remove n e1) (remove n e2)"
+    | "remove n (Cat e1 e2) = Cat (remove n e1) (remove n e2)"
+    | "remove n (Len e) = Len (remove n e)"
+    | "remove n (Let e1 e2) = Let (remove n e1) (remove (next n) e2)"
 
-primrec subst' :: "nat => expr => expr => expr"
+primrec subst' :: "var => expr => expr => expr"
 where "subst' n e' (Var v) = (if v = n then e' else Var v)"
     | "subst' n e' (Num x) = Num x"
     | "subst' n e' (Str s) = Str s"
@@ -65,73 +65,24 @@ where "subst' n e' (Var v) = (if v = n then e' else Var v)"
     | "subst' n e' (Times e1 e2) = Times (subst' n e' e1) (subst' n e' e2)"
     | "subst' n e' (Cat e1 e2) = Cat (subst' n e' e1) (subst' n e' e2)"
     | "subst' n e' (Len e) = Len (subst' n e' e)"
-    | "subst' n e' (Let e1 e2) = Let (subst' n e' e1) (subst' (Suc n) (incr_from 0 e') e2)"
+    | "subst' n e' (Let e1 e2) = Let (subst' n e' e1) (subst' (next n) (insert first e') e2)"
 
 definition subst :: "expr => expr => expr"
-where "subst e' e = sub_from 0 (subst' 0 (incr_from 0 e') e)"
+where "subst e' e = remove first (subst' first (insert first e') e)"
 
-primrec free_vars :: "expr => nat set"
-where "free_vars (Var v) = {v}"
-    | "free_vars (Num x) = {}"
-    | "free_vars (Str s) = {}"
-    | "free_vars (Plus e1 e2) = free_vars e1 Un free_vars e2"
-    | "free_vars (Times e1 e2) = free_vars e1 Un free_vars e2"
-    | "free_vars (Cat e1 e2) = free_vars e1 Un free_vars e2"
-    | "free_vars (Len e) = free_vars e"
-    | "free_vars (Let e1 e2) = free_vars e1 Un (%x. x - 1) ` (free_vars e2 - {0})"
+lemma [simp]: "typecheck gam e t ==> n in gam ==> 
+         typecheck (extend_at n gam t') (insert n e) t"
+by (induction gam e t arbitrary: n rule: typecheck.induct, fastforce+)
 
-lemma [simp]: "typecheck gam e t ==> n <= size gam ==> 
-         typecheck (extend_at n gam t') (incr_from n e) t"
-proof (induction gam e t arbitrary: n rule: typecheck.induct)
-case (tc_var x t)
-  thus ?case by simp
-next case tc_str
-  thus ?case by simp
-next case tc_num
-  thus ?case by simp
-next case tc_plus
-  thus ?case by simp
-next case tc_times
-  thus ?case by simp
-next case tc_cat
-  thus ?case by simp
-next case tc_len
-  thus ?case by simp
-next case (tc_let gam e1 t1 e2 t2)
-  from tc_let have X: "typecheck (extend_at n gam t') (incr_from n e1) t1" by simp
-  from tc_let have "typecheck (extend (extend_at n gam t') t1) (incr_from (Suc n) e2) t2" by simp
-  with X show ?case by simp
-qed
-
-lemma [simp]: "sub_from n (incr_from n e) = e"
+lemma [simp]: "remove n (insert n e) = e"
 by (induction e arbitrary: n, simp_all)
 
-lemma [simp]: "m <= n ==> incr_from m (incr_from n e) = incr_from (Suc n) (incr_from m e)"
+lemma [simp]: "canswap m n ==> insert m (insert n e) = insert (next n) (insert m e)"
 by (induction e arbitrary: n m, simp_all)
 
-lemma [simp]: "typecheck (extend_at n gam t') e t ==> n <= size gam ==> typecheck gam e' t' ==> 
-        typecheck gam (sub_from n (subst' n (incr_from n e') e)) t"
-proof (induction "extend_at n gam t'" e t arbitrary: n gam t' e' rule: typecheck.induct)
-case (tc_var x t)
-  thus ?case by auto
-next case tc_str
-  thus ?case by simp
-next case tc_num
-  thus ?case by simp
-next case tc_plus
-  thus ?case by simp
-next case tc_times
-  thus ?case by simp
-next case tc_cat
-  thus ?case by simp
-next case tc_len
-  thus ?case by simp
-next case (tc_let e1 t1 e2 t2 n)
-  with tc_let have X: "typecheck (extend gam t1) (sub_from (Suc n) (subst' (Suc n) 
-                             (incr_from (Suc n) (incr_from 0 e')) e2)) t2" by simp
-  from tc_let have "typecheck gam (sub_from n (subst' n (incr_from n e') e1)) t1" by simp
-  with X show ?case by simp
-qed
+lemma [simp]: "typecheck (extend_at n gam t') e t ==> n in gam ==> typecheck gam e' t' ==> 
+        typecheck gam (remove n (subst' n (insert n e') e)) t"
+by (induction "extend_at n gam t'" e t arbitrary: n gam t' e' rule: typecheck.induct, fastforce+)
 
 lemma [simp]: "typecheck (extend gam t') e t ==> typecheck gam e' t' ==> 
                           typecheck gam (subst e' e) t"
