isabelle/DeBruijnEnvironment.thy
@@ -2,41 +2,64 @@ theory DeBruijnEnvironment
 imports Main
 begin
 
+datatype var = DBVar nat
+
+definition first :: var
+where "first = DBVar 0"
+
+primrec "next" :: "var => var"
+where "next (DBVar v) = DBVar (Suc v)"
+
+fun incr :: "var => var => var"
+where "incr (DBVar n) (DBVar v) = DBVar (if v < n then v else Suc v)" 
+
+fun subr :: "var => var => var"
+where "subr (DBVar n) (DBVar v) = DBVar (if v < n then v else v - 1)" 
+
 datatype 'a env = DBEnv "'a list"
 
 definition empty_env :: "'a env"
 where "empty_env = DBEnv []"
 
-primrec size :: "'a env => nat"
-where "size (DBEnv as) = length as"
+fun is_in :: "var => 'a env => bool" (infix "in" 65)
+where "is_in (DBVar n) (DBEnv as) = (n <= length as)"
 
 fun lookup' :: "'a list => nat => 'a option"
 where "lookup' [] n = None"
     | "lookup' (a # as) 0 = Some a"
     | "lookup' (a # as) (Suc n) = lookup' as n"
 
-primrec lookup :: "'a env => nat => 'a option"
-where "lookup (DBEnv as) n = lookup' as n"
+fun lookup :: "'a env => var => 'a option"
+where "lookup (DBEnv as) (DBVar n) = lookup' as n"
 
 fun extend_at' :: "nat => 'a list => 'a => 'a list"
 where "extend_at' 0 as a' = a' # as"
     | "extend_at' (Suc n) [] a' = undefined"
     | "extend_at' (Suc n) (a # as) a' = a # extend_at' n as a'"
 
-primrec extend_at :: "nat => 'a env => 'a => 'a env"
-where "extend_at n (DBEnv as) a' = DBEnv (extend_at' n as a')"
+fun extend_at :: "var => 'a env => 'a => 'a env"
+where "extend_at (DBVar n) (DBEnv as) a' = DBEnv (extend_at' n as a')"
 
 abbreviation extend :: "'a env => 'a => 'a env"
-where "extend == extend_at 0"
+where "extend == extend_at first"
+
+lemma [simp]: "first in gam"
+by (induction gam, simp add: first_def)
+
+lemma [simp]: "x <= length list ==> length (extend_at' x list y) = Suc (length list)"
+by (induction x list y rule: extend_at'.induct, simp_all)
+
+lemma [simp]: "x in gam ==> n in gam ==> next n in extend_at x gam y"
+by (induction gam, induction x, induction n, simp)
+
+lemma [simp]: "subr n (incr n var) = var"
+by (induction n, induction var, simp)
 
 lemma [simp]: "lookup empty_env x = None"
-by (simp add: empty_env_def)
+by (cases x, simp add: empty_env_def)
 
 lemma [simp]: "n <= length l ==> length (extend_at' n l a) = Suc (length l)"
 by (induction n l a rule: extend_at'.induct, simp_all)
-
-lemma [simp]: "n <= size env ==> size (extend_at n env a) = Suc (size env)"
-by (induction env, simp)
 
 lemma [simp]: "n <= length l ==> lookup' (extend_at' n l t) x = 
                   (if x < n then lookup' l x else if x > n then lookup' l (x - 1) else Some t)"
@@ -55,22 +78,16 @@ next case 3
   qed
 qed
 
-lemma [simp]: "n <= size gam ==> x ~= n ==> 
-          lookup (extend_at n gam t) x = lookup gam (if x < n then x else x - 1)"
-by (induction gam, simp)
+lemma [simp]: "n in gam ==> x ~= n ==> 
+          lookup (extend_at n gam t) x = lookup gam (subr n x)"
+by (induction gam, induction n, induction x, simp)
 
-lemma [simp]: "n <= size gam ==> lookup (extend_at n gam t) n = Some t"
-by (induction gam, simp)
+lemma [simp]: "n in gam ==> lookup (extend_at n gam t) n = Some t"
+by (induction gam, induction n, simp)
 
-lemma [simp]: "ALL x : (%x. x - Suc 0) ` (s - {0}). lookup gam x = lookup gam' x ==> 
-                    ALL x : s. lookup (extend_at 0 gam t1) x = lookup (extend_at 0 gam' t1) x"
-proof (induction gam, induction gam', auto)
-  fix list::"'a list" 
-  fix lista x
-  assume "ALL x : s - {0}. lookup' lista (x - Suc 0) = lookup' list (x - Suc 0)"
-     and "x : s"
-  thus "lookup' (t1 # lista) x = lookup' (t1 # list) x" by (induction x, simp, force)
-qed
+lemma [simp]: "n in gam ==> lookup gam x = Some t ==> 
+         lookup (extend_at n gam t') (incr n x) = Some t"
+by (induction gam, induction n, induction x, simp)
 
 lemma [simp]: "n <= length l ==> m <= n ==> 
           extend_at' m (extend_at' n l a) b = extend_at' (Suc n) (extend_at' m l b) a"
@@ -83,8 +100,23 @@ next case (3 n a' as a)
   thus ?case by (cases m, simp_all)
 qed
 
-lemma [simp]: "n <= size gam ==> m <= n ==> 
-        extend_at m (extend_at n gam a) b = extend_at (Suc n) (extend_at m gam b) a"
-by (induction gam, simp)
+fun canswap :: "var => var => bool"
+where "canswap (DBVar m) (DBVar n) = (m <= n)" 
+
+lemma [simp]: "n in gam ==> canswap m n ==>
+        extend_at m (extend_at n gam a) b = extend_at (next n) (extend_at m gam b) a"
+by (induction gam, induction n, induction m, simp)
+
+lemma [simp]: "canswap m n ==> incr m (incr n var) = incr (next n) (incr m var)"
+by (induction var, induction n, induction m, simp)
+
+lemma [simp]: "canswap first x"
+by (induction x, simp add: first_def)
+
+lemma [simp]: "canswap m n ==> canswap (next m) (next n)"
+by (induction n, induction m, simp)
+
+lemma [simp]: "n in gam ==> canswap m n ==> m in gam"
+by (induction gam, induction n, induction m, simp)
 
 end
